ott/coq/AilTyping_defns.v
@@ -1,0 +1,594 @@
+Require Import Common.
+Require Import AilTypes.
+Require Import AilSyntax.
+Require Import AilTypesAux AilTypesAux_defns.
+Require Import AilSyntaxAux_defns.
+Require Import Implementation.
+Require Import Context_defns.
+Require Import AilWf_defns.
+
+Inductive wellTypedBinaryArithmetic : ctype -> arithmeticOperator -> ctype -> Prop :=    (* defn eType *)
+ | WellTypedBinaryArithmetic_Mul :
+     forall {t1 t2},
+       arithmetic t1 ->
+       arithmetic t2 ->
+       wellTypedBinaryArithmetic t1 Mul t2
+ | WellTypedBinaryArithmetic_Div :
+     forall {t1 t2},
+       arithmetic t1 ->
+       arithmetic t2 ->
+       wellTypedBinaryArithmetic t1 Div t2
+ | WellTypedBinaryArithmetic_Mod :
+     forall {t1 t2},
+       integer t1 ->
+       integer t2 ->
+       wellTypedBinaryArithmetic t1 Mod t2
+ | WellTypedBinaryArithmetic_AddArithmetic : forall (t1 t2:ctype),
+     forall {t1 t2},
+       arithmetic t1 ->
+       arithmetic t2 ->
+       wellTypedBinaryArithmetic t1 Add t2
+ | WellTypedBinaryArithmetic_SubArithmetic :
+     forall {t1 t2},
+       arithmetic t1 ->
+       arithmetic t2 ->
+       wellTypedBinaryArithmetic t1 Sub t2
+ | WellTypedBinaryArithmetic_ShiftL :
+     forall {t1 t2},
+       integer t1 ->
+       integer t2 ->
+       wellTypedBinaryArithmetic t1 Shl t2
+ | WellTypedBinaryArithmetic_ShiftR :
+     forall {t1 t2},
+       integer t1 ->
+       integer t2 ->
+       wellTypedBinaryArithmetic t1 Shr t2
+ | WellTypedBinaryArithmetic_Band :
+     forall {t1 t2},
+       integer t1 ->
+       integer t2 ->
+       wellTypedBinaryArithmetic t1 Band t2
+ | WellTypedBinaryArithmetic_Xor :
+     forall {t1 t2},
+       integer t1 ->
+       integer t2 ->
+       wellTypedBinaryArithmetic t1 Xor t2
+ | WellTypedBinaryArithmetic_Bor :
+     forall {t1 t2},
+       integer t1 ->
+       integer t2 ->
+       wellTypedBinaryArithmetic t1 Bor t2.
+
+Inductive typeOfConstant : implementation -> integerConstant -> integerType -> Prop :=
+ | TypeOfConstant_NoneInt P : forall (n:nat),
+     inIntegerRange P n (Signed Int) ->
+     typeOfConstant P (n , None) (Signed Int)
+ | TypeOfConstant_NoneLong P : forall (n:nat),
+     ~ inIntegerRange P n (Signed Int)  ->
+     inIntegerRange P n (Signed Long) ->
+     typeOfConstant P (n , None) (Signed Long)
+ | TypeOfConstant_NoneLongLong P : forall (n:nat),
+     ~ inIntegerRange P n (Signed Long)  ->
+     inIntegerRange P n (Signed LongLong) ->
+     typeOfConstant P (n , None) (Signed LongLong)
+ | TypeOfConstant_UInt P : forall (n:nat),
+     inIntegerRange P n (Unsigned Int) ->
+     typeOfConstant P (n , Some U) (Unsigned Int)
+ | TypeOfConstant_ULong P : forall (n:nat),
+     ~ inIntegerRange P n (Unsigned Int)  ->
+     inIntegerRange P n (Unsigned Long) ->
+     typeOfConstant P (n , Some U) (Unsigned Long)
+ | TypeOfConstant_ULongLong P : forall (n:nat),
+     ~ inIntegerRange P n (Unsigned Long)  ->
+     inIntegerRange P n (Unsigned LongLong) ->
+     typeOfConstant P (n , Some U) (Unsigned LongLong)
+ | TypeOfConstant_LLong P : forall (n:nat),
+     inIntegerRange P n (Signed Long) ->
+     typeOfConstant P (n , Some L) (Signed Long)
+ | TypeOfConstant_LLongLong P : forall (n:nat),
+     ~ inIntegerRange P n (Signed Long)  ->
+     inIntegerRange P n (Signed LongLong) ->
+     typeOfConstant P (n , Some L) (Signed LongLong)
+ | TypeOfConstant_ULLong P : forall (n:nat),
+     inIntegerRange P n (Unsigned Long) ->
+     typeOfConstant P (n , Some UL) (Unsigned Long)
+ | TypeOfConstant_ULLongLong P : forall (n:nat),
+     ~ inIntegerRange P n (Unsigned Long)  ->
+     inIntegerRange P n (Unsigned LongLong) ->
+     typeOfConstant P (n , Some UL) (Unsigned LongLong)
+ | TypeOfConstant_LLLongLong P : forall (n:nat),
+     inIntegerRange P n (Signed LongLong) ->
+     typeOfConstant P (n , Some LL) (Signed LongLong)
+ | TypeOfConstant_ULLLongLong P : forall (n:nat),
+     inIntegerRange P n (Unsigned LongLong) ->
+     typeOfConstant P (n , Some ULL) (Unsigned LongLong).
+
+Inductive typeOfExpression' {A B} {P} {G} {S : sigma A B} : expression' B -> typeCategory -> Prop :=    (* defn typeOfExpression' *)
+ | TypeOfExpression'_Variable : forall (v:identifier) (q:qualifiers) (t:ctype),
+     lookup G v (q, t)  ->
+     typeOfExpression' (Var v) (LValueType q t)
+ | TypeOfExpression'_Function : forall (v:identifier) (t:ctype) p,
+     lookup S v p ->
+     type_from_sigma p = t ->
+     typeOfExpression' (Var v) (RValueType t)
+ | TypeOfExpression'_Constant : forall ic it,
+     typeOfConstant P ic it ->
+     typeOfExpression' (Constant (ConstantInteger ic)) (RValueType (Basic (Integer it)))
+ | TypeOfExpression'_Call : forall es p e q t,
+     unqualified q ->
+     typeOfRValue e (Pointer q (Function t p)) ->
+     typeOfArguments es p ->
+     typeOfExpression' (Call e es) (RValueType t)
+ | TypeOfExpression'_AddressFunction : forall p e q t,
+     typeOfExpression e (RValueType (Function t p)) ->
+     unqualified q ->
+     typeOfExpression' (Unary Address e) (RValueType (Pointer q (Function t p)))
+ | TypeOfExpression'_AddressLvalue : forall e (q:qualifiers) (t:ctype),
+     typeOfLValue e q t ->
+     typeOfExpression' (Unary Address e) (RValueType (Pointer q t))
+ | TypeOfExpression'_IndirectionObject : forall e (q:qualifiers) (t:ctype),
+     typeOfRValue e (Pointer q t) ->
+     complete t ->
+     object t ->
+     typeOfExpression' (Unary Indirection e) (LValueType q t)
+ | TypeOfExpression'_IndirectionFunction : forall p e q (t:ctype),
+     unqualified q ->
+     typeOfRValue e (Pointer q (Function t p)) ->
+     typeOfExpression' (Unary Indirection e) (RValueType (Pointer q (Function t p)))
+ | TypeOfExpression'_PostfixIncrementPointer : forall e (t:ctype) (q':qualifiers) (t':ctype),
+     typeOfLValue e q' t' ->
+     lvalueConversion t' t ->
+     pointer t' ->
+     modifiable q' t' ->
+     typeOfExpression' (Unary PostfixIncr e) (RValueType t)
+ | TypeOfExpression'_PostfixIncrementReal : forall e (t:ctype) (q':qualifiers) (t':ctype),
+     typeOfLValue e q' t' ->
+     lvalueConversion t' t ->
+     real t' ->
+     modifiable q' t' ->
+     typeOfExpression' (Unary PostfixIncr e) (RValueType t)
+ | TypeOfExpression'_PostfixDecrementPointer : forall e (t:ctype) (q':qualifiers) (t':ctype),
+     typeOfLValue e q' t' ->
+     lvalueConversion t' t ->
+     pointer t' ->
+     modifiable q' t' ->
+     typeOfExpression' (Unary PostfixDecr e) (RValueType t)
+ | TypeOfExpression'_PostfixDecrementReal : forall e (t:ctype) (q':qualifiers) (t':ctype),
+     typeOfLValue e q' t' ->
+     lvalueConversion t' t ->
+     real t' ->
+     modifiable q' t' ->
+     typeOfExpression' (Unary PostfixDecr e) (RValueType t)
+ | TypeOfExpression'_Plus : forall e (t t':ctype),
+     typeOfRValue e t' ->
+     arithmetic t' ->
+     promotion P t' t ->
+     typeOfExpression' (Unary Plus e) (RValueType t)
+ | TypeOfExpression'_Minus : forall e (t t':ctype),
+     typeOfRValue e t' ->
+     arithmetic t' ->
+     promotion P t' t ->
+     typeOfExpression' (Unary Minus e) (RValueType t)
+ | TypeOfExpression'_Bnot : forall e (t t':ctype),
+     typeOfRValue e t' ->
+     integer t' ->
+     promotion P t' t ->
+     typeOfExpression' (Unary Bnot e) (RValueType t)
+ | TypeOfExpression'_SizeOf : forall (q:qualifiers) (t t':ctype),
+     wfLvalue q t ->
+     neg (function t) ->
+     neg (incomplete t) ->
+     Basic (Integer (size_t P)) = t' ->
+     typeOfExpression' (SizeOf q t) (RValueType t')
+ | TypeOfExpression'_AlignOf : forall (q:qualifiers) (t t':ctype),
+     wfLvalue q t ->
+     neg (function t) ->
+     neg (incomplete t) ->
+     Basic (Integer (size_t P)) = t' ->
+     typeOfExpression' (AlignOf q t) (RValueType t')
+ | TypeOfExpression'_CastScalar : forall (q:qualifiers) (t:ctype) e (t':ctype),
+     wfLvalue q t ->
+     typeOfRValue e t' ->
+     scalar t' ->
+     scalar t ->
+     typeOfExpression' (Cast q t e) (RValueType t)
+ | TypeOfExpression'_CastVoid : forall (q:qualifiers) e (t:ctype),
+     wfLvalue q Void ->
+     typeOfRValue e t ->
+     typeOfExpression' (Cast q Void e) (RValueType Void)
+ | TypeOfExpression'_Mul : forall e1 e2 (t t1 t2:ctype),
+     typeOfRValue e1 t1 ->
+     typeOfRValue e2 t2 ->
+     wellTypedBinaryArithmetic t1 Mul t2 ->
+     usualArithmetic P t1 t2 t ->
+     typeOfExpression' (Binary e1 (Arithmetic Mul) e2) (RValueType t)
+ | TypeOfExpression'_Div : forall e1 e2 (t t1 t2:ctype),
+     typeOfRValue e1 t1 ->
+     typeOfRValue e2 t2 ->
+     wellTypedBinaryArithmetic t1 Div t2 ->
+     usualArithmetic P t1 t2 t ->
+     typeOfExpression' (Binary e1 (Arithmetic Div) e2) (RValueType t)
+ | TypeOfExpression'_Mod : forall e1 e2 (t t1 t2:ctype),
+     typeOfRValue e1 t1 ->
+     typeOfRValue e2 t2 ->
+     wellTypedBinaryArithmetic t1 Mod t2 ->
+     usualArithmetic P t1 t2 t ->
+     typeOfExpression' (Binary e1 (Arithmetic Mod) e2) (RValueType t)
+ | TypeOfExpression'_AddArithmetic : forall e1 e2 (t t1 t2:ctype),
+     typeOfRValue e1 t1 ->
+     typeOfRValue e2 t2 ->
+     wellTypedBinaryArithmetic t1 Add t2 ->
+     usualArithmetic P t1 t2 t ->
+     typeOfExpression' (Binary e1 (Arithmetic Add) e2) (RValueType t)
+ | TypeOfExpression'_AddPointer1 : forall e1 e2 (q1:qualifiers) (t1 t2:ctype),
+     typeOfRValue e1 (Pointer q1 t1) ->
+     typeOfRValue e2 t2 ->
+     complete t1 ->
+     integer t2 ->
+     typeOfExpression' (Binary e1 (Arithmetic Add) e2) (RValueType (Pointer q1 t1))
+ | TypeOfExpression'_AddPointer2 : forall e1 e2 (q2:qualifiers) (t2 t1:ctype),
+     typeOfRValue e1 t1 ->
+     typeOfRValue e2 (Pointer q2 t2) ->
+     integer t1 ->
+     complete t2 ->
+     typeOfExpression' (Binary e1 (Arithmetic Add) e2) (RValueType (Pointer q2 t2))
+ | TypeOfExpression'_SubArithmetic : forall e1 e2 (t t1 t2:ctype),
+     typeOfRValue e1 t1 ->
+     typeOfRValue e2 t2 ->
+     wellTypedBinaryArithmetic t1 Sub t2 ->
+     usualArithmetic P t1 t2 t ->
+     typeOfExpression' (Binary e1 (Arithmetic Sub) e2) (RValueType t)
+ | TypeOfExpression'_SubPointer : forall e1 e2 (q1:qualifiers) (t1 t2:ctype),
+     typeOfRValue e1 (Pointer q1 t1) ->
+     typeOfRValue e2 t2 ->
+     complete t1 ->
+     integer t2 ->
+     typeOfExpression' (Binary e1 (Arithmetic Sub) e2) (RValueType (Pointer q1 t1))
+ | TypeOfExpression'_SubPointerDiff : forall e1 e2 (t:ctype) (q1:qualifiers) (t1:ctype) (q2:qualifiers) (t2:ctype),
+     typeOfRValue e1 (Pointer q1 t1) ->
+     typeOfRValue e2 (Pointer q2 t2) ->
+     complete t1 ->
+     complete t2 ->
+     compatible t1 t2 ->
+     Basic (Integer (ptrdiff_t P)) = t ->
+     typeOfExpression' (Binary e1 (Arithmetic Sub) e2) (RValueType t)
+ | TypeOfExpression'_ShiftL : forall e1 e2 (t1' t1 t2:ctype),
+     typeOfRValue e1 t1 ->
+     typeOfRValue e2 t2 ->
+     wellTypedBinaryArithmetic t1 Shl t2 ->
+     promotion P t1 t1' ->
+     typeOfExpression' (Binary e1 (Arithmetic Shl) e2) (RValueType t1')
+ | TypeOfExpression'_ShiftR : forall e1 e2 (t1' t1 t2:ctype),
+     typeOfRValue e1 t1 ->
+     typeOfRValue e2 t2 ->
+     wellTypedBinaryArithmetic t1 Shr t2 ->
+     promotion P t1 t1' ->
+     typeOfExpression' (Binary e1 (Arithmetic Shr) e2) (RValueType t1')
+ | TypeOfExpression'_LtReal : forall e1 e2 (t1 t2:ctype),
+     typeOfRValue e1 t1 ->
+     typeOfRValue e2 t2 ->
+     real t1 ->
+     real t2 ->
+     typeOfExpression' (Binary e1 Lt e2) (RValueType (Basic (Integer (Signed Int))) )
+ | TypeOfExpression'_LtPointer : forall e1 e2 (q1:qualifiers) (t1:ctype) (q2:qualifiers) (t2:ctype),
+     typeOfRValue e1 (Pointer q1 t1) ->
+     typeOfRValue e2 (Pointer q2 t2) ->
+     object t1 ->
+     object t2 ->
+     compatible t1 t2 ->
+     typeOfExpression' (Binary e1 Lt e2) (RValueType (Basic (Integer (Signed Int))) )
+ | TypeOfExpression'_GtReal : forall e1 e2 (t1 t2:ctype),
+     typeOfRValue e1 t1 ->
+     typeOfRValue e2 t2 ->
+     real t1 ->
+     real t2 ->
+     typeOfExpression' (Binary e1 Gt e2) (RValueType (Basic (Integer (Signed Int))) )
+ | TypeOfExpression'_GtPointer : forall e1 e2 (q1:qualifiers) (t1:ctype) (q2:qualifiers) (t2:ctype),
+     typeOfRValue e1 (Pointer q1 t1) ->
+     typeOfRValue e2 (Pointer q2 t2) ->
+     object t1 ->
+     object t2 ->
+     compatible t1 t2 ->
+     typeOfExpression' (Binary e1 Gt e2) (RValueType (Basic (Integer (Signed Int))) )
+ | TypeOfExpression'_LeReal : forall e1 e2 (t1 t2:ctype),
+     typeOfRValue e1 t1 ->
+     typeOfRValue e2 t2 ->
+     real t1 ->
+     real t2 ->
+     typeOfExpression' (Binary e1 Le e2) (RValueType (Basic (Integer (Signed Int))) )
+ | TypeOfExpression'_LePointer : forall e1 e2 (q1:qualifiers) (t1:ctype) (q2:qualifiers) (t2:ctype),
+     typeOfRValue e1 (Pointer q1 t1) ->
+     typeOfRValue e2 (Pointer q2 t2) ->
+     object t1 ->
+     object t2 ->
+     compatible t1 t2 ->
+     typeOfExpression' (Binary e1 Le e2) (RValueType (Basic (Integer (Signed Int))) )
+ | TypeOfExpression'_GeReal : forall e1 e2 (t1 t2:ctype),
+     typeOfRValue e1 t1 ->
+     typeOfRValue e2 t2 ->
+     real t1 ->
+     real t2 ->
+     typeOfExpression' (Binary e1 Ge e2) (RValueType (Basic (Integer (Signed Int))) )
+ | TypeOfExpression'_GePointer : forall e1 e2 (q1:qualifiers) (t1:ctype) (q2:qualifiers) (t2:ctype),
+     typeOfRValue e1 (Pointer q1 t1) ->
+     typeOfRValue e2 (Pointer q2 t2) ->
+     object t1 ->
+     object t2 ->
+     compatible t1 t2 ->
+     typeOfExpression' (Binary e1 Ge e2) (RValueType (Basic (Integer (Signed Int))) )
+ | TypeOfExpression'_EqArithmetic : forall e1 e2 (t1 t2:ctype),
+     typeOfRValue e1 t1 ->
+     typeOfRValue e2 t2 ->
+     arithmetic t1 ->
+     arithmetic t2 ->
+     typeOfExpression' (Binary e1 Eq e2) (RValueType (Basic (Integer (Signed Int))) )
+ | TypeOfExpression'_EqPointer : forall e1 e2 (q1:qualifiers) (t1:ctype) (q2:qualifiers) (t2:ctype),
+     typeOfRValue e1 (Pointer q1 t1) ->
+     typeOfRValue e2 (Pointer q2 t2) ->
+     compatible t1 t2 ->
+     typeOfExpression' (Binary e1 Eq e2) (RValueType (Basic (Integer (Signed Int))) )
+ | TypeOfExpression'_EqVoid1 : forall e1 e2 (q1 q2:qualifiers) (t2:ctype),
+     typeOfRValue e1 (Pointer q1 Void) ->
+     typeOfRValue e2 (Pointer q2 t2) ->
+     object t2 ->
+     typeOfExpression' (Binary e1 Eq e2) (RValueType (Basic (Integer (Signed Int))) )
+ | TypeOfExpression'_EqVoid2 : forall e1 e2 (q1:qualifiers) (t1:ctype) (q2:qualifiers),
+     typeOfRValue e1 (Pointer q1 t1) ->
+     typeOfRValue e2 (Pointer q2 Void) ->
+     object t1 ->
+     typeOfExpression' (Binary e1 Eq e2) (RValueType (Basic (Integer (Signed Int))) )
+ | TypeOfExpression'_EqNull1 : forall e1 e2 (t1:ctype) (q2:qualifiers) (t2:ctype),
+     typeOfRValue e1 t1 ->
+     typeOfRValue e2 (Pointer q2 t2) ->
+     nullPointerConstant e1 ->
+     typeOfExpression' (Binary e1 Eq e2) (RValueType (Basic (Integer (Signed Int))) )
+ | TypeOfExpression'_EqNull2 : forall e1 e2 (q1:qualifiers) (t1 t2:ctype),
+     typeOfRValue e1 (Pointer q1 t1) ->
+     typeOfRValue e2 t2 ->
+     nullPointerConstant e2 ->
+     typeOfExpression' (Binary e1 Eq e2) (RValueType (Basic (Integer (Signed Int))) )
+ | TypeOfExpression'_NeArithmetic : forall e1 e2 (t1 t2:ctype),
+     typeOfRValue e1 t1 ->
+     typeOfRValue e2 t2 ->
+     arithmetic t1 ->
+     arithmetic t2 ->
+     typeOfExpression' (Binary e1 Ne e2) (RValueType (Basic (Integer (Signed Int))) )
+ | TypeOfExpression'_NePointer : forall e1 e2 (q1:qualifiers) (t1:ctype) (q2:qualifiers) (t2:ctype),
+     typeOfRValue e1 (Pointer q1 t1) ->
+     typeOfRValue e2 (Pointer q2 t2) ->
+     compatible t1 t2 ->
+     typeOfExpression' (Binary e1 Ne e2) (RValueType (Basic (Integer (Signed Int))) )
+ | TypeOfExpression'_NeVoid1 : forall e1 e2 (q1 q2:qualifiers) (t2:ctype),
+     typeOfRValue e1 (Pointer q1 Void) ->
+     typeOfRValue e2 (Pointer q2 t2) ->
+     object t2 ->
+     typeOfExpression' (Binary e1 Ne e2) (RValueType (Basic (Integer (Signed Int))) )
+ | TypeOfExpression'_NeVoid2 : forall e1 e2 (q1:qualifiers) (t1:ctype) (q2:qualifiers),
+     typeOfRValue e1 (Pointer q1 t1) ->
+     typeOfRValue e2 (Pointer q2 Void) ->
+     object t1 ->
+     typeOfExpression' (Binary e1 Ne e2) (RValueType (Basic (Integer (Signed Int))) )
+ | TypeOfExpression'_NeNull1 : forall e1 e2 (t1:ctype) (q2:qualifiers) (t2:ctype),
+     typeOfRValue e1 t1 ->
+     typeOfRValue e2 (Pointer q2 t2) ->
+     nullPointerConstant e1 ->
+     typeOfExpression' (Binary e1 Ne e2) (RValueType (Basic (Integer (Signed Int))) )
+ | TypeOfExpression'_NeNull2 : forall e1 e2 (q1:qualifiers) (t1 t2:ctype),
+     typeOfRValue e1 (Pointer q1 t1) ->
+     typeOfRValue e2 t2 ->
+     nullPointerConstant e2 ->
+     typeOfExpression' (Binary e1 Ne e2) (RValueType (Basic (Integer (Signed Int))) )
+ | TypeOfExpression'_Band : forall e1 e2 (t t1 t2:ctype),
+     typeOfRValue e1 t1 ->
+     typeOfRValue e2 t2 ->
+     wellTypedBinaryArithmetic t1 Band t2 ->
+     usualArithmetic P t1 t2 t ->
+     typeOfExpression' (Binary e1 (Arithmetic Band) e2) (RValueType t)
+ | TypeOfExpression'_Xor : forall e1 e2 (t t1 t2:ctype),
+     typeOfRValue e1 t1 ->
+     typeOfRValue e2 t2 ->
+     wellTypedBinaryArithmetic t1 Xor t2 ->
+     usualArithmetic P t1 t2 t ->
+     typeOfExpression' (Binary e1 (Arithmetic Xor) e2) (RValueType t)
+ | TypeOfExpression'_Bor : forall e1 e2 (t t1 t2:ctype),
+     typeOfRValue e1 t1 ->
+     typeOfRValue e2 t2 ->
+     wellTypedBinaryArithmetic t1 Bor t2 ->
+     usualArithmetic P t1 t2 t ->
+     typeOfExpression' (Binary e1 (Arithmetic Bor) e2) (RValueType t)
+ | TypeOfExpression'_And : forall e1 e2 (t1 t2:ctype),
+     typeOfRValue e1 t1 ->
+     typeOfRValue e2 t2 ->
+     scalar t1 ->
+     scalar t2 ->
+     typeOfExpression' (Binary e1 And e2) (RValueType (Basic (Integer (Signed Int))) )
+ | TypeOfExpression'_Or : forall e1 e2 (t1 t2:ctype),
+     typeOfRValue e1 t1 ->
+     typeOfRValue e2 t2 ->
+     scalar t1 ->
+     scalar t2 ->
+     typeOfExpression' (Binary e1 Or e2) (RValueType (Basic (Integer (Signed Int))) )
+ | TypeOfExpression'_ConditionalArithmetic : forall e1 e2 e3 (t t1 t2 t3:ctype),
+     typeOfRValue e1 t1 ->
+     scalar t1 ->
+     typeOfRValue e2 t2 ->
+     typeOfRValue e3 t3 ->
+     arithmetic t2 ->
+     arithmetic t3 ->
+     usualArithmetic P t2 t3 t ->
+     typeOfExpression' (Conditional e1 e2 e3) (RValueType t)
+ | TypeOfExpression'_ConditionalVoid : forall e1 e2 e3 (t1:ctype),
+     typeOfRValue e1 t1 ->
+     scalar t1 ->
+     typeOfRValue e2 Void ->
+     typeOfRValue e3 Void ->
+     typeOfExpression' (Conditional e1 e2 e3) (RValueType Void)
+ | TypeOfExpression'_ConditionalPointer : forall e1 e2 e3 (q2 q3 q:qualifiers) (t t1 t2 t3:ctype),
+     typeOfRValue e1 t1 ->
+     scalar t1 ->
+     typeOfRValue e2 (Pointer q2 t2) ->
+     typeOfRValue e3 (Pointer q3 t3) ->
+     compatible t2 t3 ->
+     composite t2 t3 t ->
+     combine_qualifiers q2 q3 = q ->
+     typeOfExpression' (Conditional e1 e2 e3) (RValueType (Pointer q t))
+ | TypeOfExpression'_ConditionalNullPointer1_Pointer : forall e1 e2 e3 (t3 t1 t2:ctype) q2 q3 q,
+     typeOfRValue e1 t1 ->
+     scalar t1 ->
+     typeOfRValue e2 (Pointer q2 t2) ->
+     typeOfRValue e3 (Pointer q3 t3) ->
+     nullPointerConstant e2 ->
+     combine_qualifiers q2 q3 = q ->
+     typeOfExpression' (Conditional e1 e2 e3) (RValueType (Pointer q t3))
+ | TypeOfExpression'_ConditionalNullPointer1_Other : forall e1 e2 e3 (t3 t1 t2:ctype),
+     typeOfRValue e1 t1 ->
+     scalar t1 ->
+     typeOfRValue e2 t2 ->
+     typeOfRValue e3 t3 ->
+     neg (pointer t2) ->
+     pointer t3 ->
+     nullPointerConstant e2 ->
+     typeOfExpression' (Conditional e1 e2 e3) (RValueType t3)
+ | TypeOfExpression'_ConditionalNullPointer2_Pointer : forall e1 e2 e3 (t2 t1 t3:ctype) q2 q3 q,
+     typeOfRValue e1 t1 ->
+     scalar t1 ->
+     typeOfRValue e2 (Pointer q2 t2) ->
+     typeOfRValue e3 (Pointer q3 t3) ->
+     nullPointerConstant e3 ->
+     combine_qualifiers q2 q3 = q ->
+     typeOfExpression' (Conditional e1 e2 e3) (RValueType (Pointer q t2))
+ | TypeOfExpression'_ConditionalNullPointer2_Other : forall e1 e2 e3 (t2 t1 t3:ctype),
+     typeOfRValue e1 t1 ->
+     scalar t1 ->
+     typeOfRValue e2 t2 ->
+     typeOfRValue e3 t3 ->
+     pointer t2 ->
+     neg (pointer t3) ->
+     nullPointerConstant e3 ->
+     typeOfExpression' (Conditional e1 e2 e3) (RValueType t2)
+ | TypeOfExpression'_ConditionalPointerVoid1 : forall e1 e2 e3 (q2 q3 q:qualifiers) (t2 t1 t3:ctype),
+     typeOfRValue e1 t1 ->
+     scalar t1 ->
+     typeOfRValue e2 (Pointer q2 t2) ->
+     typeOfRValue e3 (Pointer q3 t3) ->
+     neg (compatible t2 t3) ->
+     neg (nullPointerConstant e2) ->
+     void t2 ->
+     object t3 ->
+     combine_qualifiers q2 q3 = q ->
+     typeOfExpression' (Conditional e1 e2 e3) (RValueType (Pointer q t2))
+ | TypeOfExpression'_ConditionalPointerVoid2 : forall e1 e2 e3 (q2 q3 q:qualifiers) (t3 t1 t2:ctype),
+     typeOfRValue e1 t1 ->
+     scalar t1 ->
+     typeOfRValue e2 (Pointer q2 t2) ->
+     typeOfRValue e3 (Pointer q3 t3) ->
+     neg (compatible t2 t3) ->
+     neg (nullPointerConstant e3) ->
+     object t2 ->
+     void t3 ->
+     combine_qualifiers q2 q3 = q ->
+     typeOfExpression' (Conditional e1 e2 e3) (RValueType (Pointer q t3))
+ | TypeOfExpression'_Assign : forall e1 e2 (q1:qualifiers) (t1 t:ctype),
+     typeOfLValue e1 q1 t1 ->
+     modifiable q1 t1 ->
+     pointerConversion t1 t ->
+     assignable t e2 ->
+     typeOfExpression' (Assign e1 e2) (RValueType t)
+ | TypeOfExpression'_CompoundAssignPlusMinusArithmetic : forall aop e1 e2 (t1:ctype) (q:qualifiers) (t t2 :ctype),
+     (aop = Add) + (aop = Sub) ->
+     typeOfLValue e1 q t ->
+     lvalueConversion t t1 ->
+     typeOfRValue e2 t2 ->
+     modifiable q t ->
+     arithmetic t1 ->
+     arithmetic t2 ->
+     typeOfExpression' (CompoundAssign e1 aop e2) (RValueType t1)
+ | TypeOfExpression'_CompoundAssignPlusMinusPointer : forall aop e1 e2 (t1:ctype) (q' q:qualifiers) (t t2:ctype),
+     (aop = Add) + (aop = Sub) ->
+     typeOfLValue e1 q' (Pointer q t) ->
+     lvalueConversion (Pointer q t) t1 ->
+     typeOfRValue e2 t2 ->
+     modifiable q' (Pointer q t)  ->
+     complete t ->
+     integer t2 ->
+     typeOfExpression' (CompoundAssign e1 aop e2) (RValueType t1)
+ | TypeOfExpression'_CompoundAssign : forall aop e1 e2 (t1:ctype) (q:qualifiers) (t t2:ctype),
+     neg ((aop = Add) + (aop = Sub)) ->
+     typeOfLValue e1 q t ->
+     lvalueConversion t t1 ->
+     typeOfRValue e2 t2 ->
+     modifiable q t ->
+     wellTypedBinaryArithmetic t1 aop t2 ->
+     typeOfExpression' (CompoundAssign e1 aop e2) (RValueType t1)
+ | TypeOfExpression'_Comma : forall e1 e2 (t2 t1:ctype),
+     typeOfRValue e1 t1 ->
+     typeOfRValue e2 t2 ->
+     typeOfExpression' (Binary e1 Comma e2) (RValueType t2)
+with typeOfExpression {A B} {P} {G} {S : sigma A B} : expression B -> typeCategory -> Prop :=
+ | TypeOfExpression_Annotated : forall a e t,
+     typeOfExpression' e t ->
+     typeOfExpression (AnnotatedExpression a e) t
+with typeOfRValue {A B} {P} {G} {S : sigma A B} : expression B -> ctype -> Prop :=    (* defn typeOfRValue *)
+ | typeOfRValue_RValueType : forall e (t t':ctype),
+     typeOfExpression e (RValueType t') ->
+     pointerConversion t' t ->
+     typeOfRValue e t
+ | typeOfRValue_LValueType : forall e (t t':ctype) (q:qualifiers),
+     typeOfLValue e q t' ->
+     lvalueConversion t' t ->
+     typeOfRValue e t
+with typeOfLValue {A B} {P} {G} {S : sigma A B} : expression B -> qualifiers -> ctype -> Prop :=
+ | TypeOfLValue : forall e q t,
+     typeOfExpression e (LValueType q t) ->
+     typeOfLValue e q t
+with typeable {A B} {P} {G} {S : sigma A B} : expression B -> Prop :=    (* defn typeable *)
+ | Typeable : forall e t,
+     typeOfExpression e t ->
+     typeable e
+with typeOfArguments {A B} {P} {G} {S : sigma A B} : list (expression B) -> list (qualifiers * ctype) -> Prop :=    (* defn assignable *)
+ | TypeOfArguments_nil : typeOfArguments nil nil
+ | TypeOfArguments_cons es p : forall e q t t',
+     pointerConversion t t' ->
+     assignable t' e ->
+     typeOfArguments es p ->
+     typeOfArguments (e :: es) ((q, t) :: p)
+with assignable {A B} {P} {G} {S : sigma A B}: ctype -> expression B -> Prop :=
+ | Assignable_Arithmetic : forall e2 t1 t2,
+     typeOfRValue e2 t2 ->
+     arithmetic t1 ->
+     arithmetic t2 ->
+     assignable t1 e2
+ | Assignable_Pointer : forall e2 (q1 q2:qualifiers) (t1 t2:ctype),
+     typeOfRValue e2 (Pointer q2 t2) ->
+     compatible t1 t2 ->
+     sub_qualifiers q2 q1 = true ->
+     assignable (Pointer q1 t1) e2
+ | Assignable_VoidPointer1 : forall e2 (q1 q2:qualifiers) (t1 t2:ctype),
+     void t1 ->
+     typeOfRValue e2 (Pointer q2 t2) ->
+     object t2 ->
+     sub_qualifiers q2 q1 = true ->
+     assignable (Pointer q1 t1) e2
+ | Assignable_VoidPointer2 : forall e2 (q1 q2:qualifiers) (t1 t2:ctype),
+     object t1 ->
+     typeOfRValue e2 (Pointer q2 t2) ->
+     void t2 ->
+     sub_qualifiers q2 q1 = true ->
+     assignable (Pointer q1 t1) e2
+ | Assignable_NullPointerConstant : forall e2 (t1 t2:ctype),
+     pointer t1 ->
+     typeOfRValue e2 t2 ->
+     nullPointerConstant e2 ->
+     assignable t1 e2
+ | Assignable_Bool : forall e2 (t1 t2:ctype),
+     boolean t1 ->
+     typeOfRValue e2 t2 ->
+     pointer t2 ->
+     assignable t1 e2.
+Arguments typeOfExpression' : default implicits.
+Arguments typeOfExpression  : default implicits.
+Arguments typeOfArguments   : default implicits.
+Arguments typeOfLValue      : default implicits.
+Arguments typeOfRValue      : default implicits.
+Arguments assignable        : default implicits.
+Arguments typeable          : default implicits.
